Source/IntegrationTests/TestFiles/LitTests/LitTest/concurrency-sound/concurrency-test2.dfy
@@ -38,3 +38,90 @@ method {:volatile} ReplaceOncall(oncall: Role, name: string, age: nat)
   oncall.ReplaceWith(name, age);  // TODO: Emit locks and remove error
   assert oncall.name == name && oncall.age == age;     // Now provable
 }
+
+trait Lock {
+  ghost function threadsWithLock(): set<nat> reads this
+    decreases 0
+
+  predicate Acceptable(threadId: int)
+  
+  method {:volatile} lock(CURRENT_THREAD_ID: int)
+    requires |threadsWithLock()| <= 1
+    decreases * // Locally we can't prove something else
+    ensures Acceptable(CURRENT_THREAD_ID) ==>
+              CURRENT_THREAD_ID in threadsWithLock()
+    ensures |threadsWithLock()| <= 1 // Mutual exclusion
+
+  lemma DeadlockFree()
+
+  lemma StarvationFree()
+  
+  /*method {:volatile} unlock(CURRENT_THREAD_ID: int)
+    ensures Acceptable(CURRENT_THREAD_ID) ==>
+              CURRENT_THREAD_ID !in threadsWithLock()
+    ensures |threadsWithLock| <= old(|threadsWithLock|)
+    ensures |threadsWithLock| <= 1 // Mutual exclusivity
+    */
+}
+
+class LockOne extends Lock {
+  var flag1: bool
+  var flag2: bool
+  var test: bool
+
+  predicate Acceptable(threadId: int) {
+    0 <= threadId < 2
+  }
+
+  function flagFor(threadId: int): bool reads this
+    requires Acceptable(threadId)
+  {
+    if threadId == 0 then flag1 else flag2
+  }
+
+
+  ghost function threadsWithLock(): set<nat> reads this decreases 0 {
+    (if flag1 then {0} else {}) +
+    (if flag2 then {1} else {})
+  }
+  
+  method {:volatile} lock(CURRENT_THREAD_ID: int) decreases *
+    requires |threadsWithLock()| <= 1
+    ensures Acceptable(CURRENT_THREAD_ID) ==>
+       CURRENT_THREAD_ID in threadsWithLock()
+    ensures |threadsWithLock()| <= 1
+  {
+    if !Acceptable(CURRENT_THREAD_ID) {
+      return;
+    }
+    if CURRENT_THREAD_ID == 0 {
+      this.flag1 := true;
+    } else {
+      this.flag2 := true;
+    }
+    assert if CURRENT_THREAD_ID == 0 then flag1 else flag2;
+    assert CURRENT_THREAD_ID in threadsWithLock();
+    // TODO: control flow should enable to create only one heap.
+    var test := flagFor(1-CURRENT_THREAD_ID);
+    // Need nonlocal reasoning that can state that
+    // CURRENT_THREAD_ID stays in threadsWithLock() 
+    while test
+      invariant test == flagFor(1-CURRENT_THREAD_ID)
+        //if CURRENT_THREAD_ID == 0 then flag2 else flag1
+      decreases *
+    {
+      test := flagFor(1-CURRENT_THREAD_ID);
+    } // Autolock for read
+    assert |threadsWithLock()| <= 1;
+  }
+  lemma DeadlockFree()
+
+  lemma StarvationFree()
+  /*method {:volatile} unlock(CURRENT_THREAD_ID: int)
+    ensures CURRENT_THREAD_ID <= 1 ==>
+       CURRENT_THREAD_ID !in threadsWithLock()
+    ensures |threadsWithLock| <= 1
+  {
+    flags[CURRENT_THREAD_ID] := false;
+  }*/
+}
